worked on generic problem

theories/L/Complexity/Reductions/TMGenNP/IntermediateProblems.v
@@ -26,50 +26,70 @@ Check NPhard_GenNP.
 
 From Undecidability.L.AbstractMachines.FlatPro Require LM_heap_def LM_heap_correct LPro Decompile.
 Section LMGenNPHalt.
-  Import LM_heap_def LM_heap_correct LBool.
+  Import LM_heap_def LM_heap_correct LBool ResourceMeasures.
 
+  
   Definition initLMGen s c : (list (nat*list Tok)*list (nat*list Tok)*list (option ((nat * list Tok) * nat)))
-    := ([(0,s)],[(0,c)],[]).
+    := ([(0,s++c++[appT])],[],[]).
 
   Section fixX.
     Context (X:Type) `{R__X : registered X}.
     
     Definition LMGenNPHalt' : list Tok*nat*nat -> Prop :=
-      fun '(P, maxSize, steps (*in unary*)) =>
-        exists (c:X), size (enc c) <= maxSize /\ halts_k (initLMGen P (compile (enc c))) steps.
+      fun '(P, maxSize, k (*in unary*)) =>
+        exists (c:X), size (enc c) <= maxSize /\ (exists sigma' k', k' <= k /\ evaluatesIn step k' (initLMGen P (compile (enc c))) sigma').
 
     Definition LMHaltsOrDiverges : list Tok*nat*nat -> Prop :=
       fun '(P, maxSize, steps (*in unary*)) =>
-        (exists s, P = compile s /\ closed s)
-        /\ forall (c : X), size (enc c) <= maxSize -> forall k, halts_k (initLMGen P (compile (enc c))) k -> k <= steps.
+        (exists s, P = compile s /\ proc s)
+        /\ forall (c : X), size (enc c) <= maxSize -> forall k sigma', evaluatesIn step k (initLMGen P (compile (enc c))) sigma' -> k <= steps.
 
     Definition LMGenNPHalt := restrictBy LMHaltsOrDiverges LMGenNPHalt'.
   End fixX.
+  
   Arguments LMGenNPHalt : clear implicits.
   Arguments LMGenNPHalt _ {_}.
-  
-  From Undecidability.L Require Import Functions.LoopSum.
-  
+    
   Lemma polyRed_GenNPHalt_to_LMGenNPHalt (X:Type) `{R__X : registered X}:
     GenNPHalt X ⪯p LMGenNPHalt X.
   Proof.
-    evar (f__maxSize : nat -> nat). [f__maxSize ]:intros n0. evar (f__steps : nat -> nat). [f__steps]:intros n0.
-    pose (f := (fun '(s, maxSize, steps) => (compile s,f__maxSize maxSize, f__steps steps))).
-    eapply reducesPolyMO_intro with (f:=f). 
-
-
+    evar (f__steps : nat -> nat). [f__steps]:intros n0.
+    pose (f := (fun '(s, maxSize, steps) => (compile s,maxSize : nat, f__steps steps))).
+    eapply reducesPolyMO_intro_restrictBy with (f:=f).
+    2:{
+      intros [[s' maxSize] steps]. cbn - [GenNPHalt' LMGenNPHalt'].
+      intros (cs&Hsize). assert (lambda s') as [s0 eq] by Lproc. set (s:=lam s0) in *. subst s'.
+      split.
+      -split. easy.
+       intros c H k sigma' R__M. unfold initLMGen in R__M.
+       eapply soundnessTime with (s:=(L.app s (@enc _ R__X c))) in R__M as (g&H'&t&n&eq__sigma&Rs%timeBS_evalIn&_&eq). 2:Lproc.
+       subst k. apply Hsize in Rs. rewrite Rs. unfold f__steps. reflexivity. easy. 
+      -apply Morphisms_Prop.ex_iff_morphism. intros c.
+       apply Morphisms_Prop.and_iff_morphism_obligation_1. easy.
+       split.
+       +intros (?&(?&?&Ev)%evalLe_evalIn). eapply timeBS_evalIn,completenessTime in Ev. 2:Lproc.
+        destruct Ev as (g&Heap&?&Rs).
+        eexists _,_. split. 2:split. 2:exact Rs. now cbn; lia. now intros ? ?.
+       +intros (?&?&?&R__M).
+        eapply soundnessTime with (s:=(L.app s (@enc _ R__X c))) in R__M as (g&H'&t&n&eq__sigma&Rs%timeBS_evalIn&_&eq). 2:Lproc.
+        eexists. eapply evalIn_evalLe. 2:easy. cbn in H;nia.
+    }
+    subst f__steps;cbn beta in f.
+    evar (time : nat -> nat). [time]:intros n0.
+    exists time.
+    { unfold f. (*TODO: compile *) Fail extract.
   
-
+(*
   From Undecidability.LAM  Require TM.HaltingProblem.
   About HaltingProblem.Loop_Rel.
   About HaltingProblem.Loop_T.
-
+*)
   Abort.
 End LMGenNPHalt.
 
 
 (** Not Complete: nice form of Time bound *)
-From Undecidability.LAM  Require TM.LMBounds.
+(* From Undecidability.LAM  Require TM.LMBounds. *)
 
 
 (** Approach: simulate step-indexed L interpreter inside TM *)
